Begin doing manual inversion due to subtypes

language_formalisation/type_system/subtyping_lemmas.v
@@ -3,7 +3,7 @@ Add LoadPath "C:\Users\Ziga\Documents\Ziga_podatki\PHD\language_formalisation\ty
 Require Import syntax declarational.
 
 
-Fixpoint subty_pi A B C :
+Fixpoint subty_shape_pair A B C :
   vsubtype C (TyΠ A B) -> 
   exists A' B', C = (TyΠ A' B') /\ vsubtype A' A /\ vsubtype B' B.
 Proof.
@@ -12,21 +12,172 @@ inv orig. exists A0. exists B0.
 constructor. reflexivity. constructor; assumption.
 Qed.
 
-
-Fixpoint subty_pair Γ v1 v2 A B :
-has_vtype Γ (Pair v1 v2) (TyΠ A B) ->
-has_vtype Γ v1 A /\ has_vtype Γ v2 B.
+Fixpoint subty_shape_sum A B C :
+  vsubtype C (TyΣ A B) -> 
+  exists A' B', C = (TyΣ A' B') /\ vsubtype A' A /\ vsubtype B' B.
 Proof.
-intro orig. inv orig. inv H1. constructor; assumption.
-induction H3.
+intro orig.
+inv orig. exists A0. exists B0.
+constructor. reflexivity. constructor; assumption.
+Qed.
+
+Fixpoint subty_shape_fun A B C :
+  vsubtype C (TyFun A B) -> 
+  exists A' B', C = (TyFun A' B') /\ vsubtype A A' /\ csubtype B' B.
+Proof.
+intro orig.
+inv orig. exists A0. exists C0.
+constructor. reflexivity. constructor; assumption.
+Qed.
+
+Fixpoint subty_shape_handler A B C :
+  vsubtype C (TyHandler A B) -> 
+  exists A' B', C = (TyHandler A' B') /\ csubtype A A' /\ csubtype B' B.
+Proof.
+intro orig.
+inv orig. exists C0. exists D.
+constructor. reflexivity. constructor; assumption.
+Qed.
 
 
-intro orig. inv orig. inv H1. constructor; assumption.
-apply subty_pi in H3. destruct H3. destruct H1. destruct H1.
-subst. apply subty_pair in H2.
-destruct H2. destruct H3. constructor.
-- apply TypeV. assumption. inv H0. assumption.
-  eapply TypeVSubtype. exact H1. assumption.
-- apply TypeV. assumption. inv H0. assumption.
-  eapply TypeVSubtype. exact H2. assumption.
+Fixpoint shape_pair_full Γ v A B ty (orig : has_vtype Γ v ty) {struct orig} :
+  ty = TyΠ A B ->
+  (exists name num, v = Var (name, num)) \/
+  (exists v1 v2, v = Pair v1 v2 /\ has_vtype Γ v1 A /\ has_vtype Γ v2 B).
+Proof.
+intros same.
+destruct orig. destruct H1; try discriminate.
++ clear shape_pair_full. left. exists name. exists num. reflexivity.
++ clear shape_pair_full. right. exists v1. exists v2. 
+  constructor. reflexivity. injection same. intros. subst. 
+  constructor; assumption.
++ rewrite same in H2. apply subty_shape_pair in H2. 
+  destruct H2 as [A'' [B'' [pity]]]. subst. 
+  apply (shape_pair_full _ _ A'' B'') in H1. clear shape_pair_full. 
+  2: reflexivity. destruct H1.
+  - left. assumption.
+  - right. destruct H1 as [v1 [v2]]. exists v1. exists v2.
+    constructor. destruct H1. assumption.
+    constructor; destruct H1; destruct H3; destruct H2;
+    apply TypeV; inv H0; try assumption. 
+    * eapply TypeVSubtype. exact H3. assumption.
+    * eapply TypeVSubtype. exact H4. assumption.
+Qed.
+
+Lemma shape_pair Γ v1 v2 A B :
+  has_vtype Γ (Pair v1 v2) (TyΠ A B) ->  
+  has_vtype Γ v1 A /\ has_vtype Γ v2 B.
+Proof.
+intro orig.
+apply (shape_pair_full _ _ A B) in orig as shape. 2: reflexivity.
+destruct shape.
++ destruct H as [name [num]]. discriminate.
++ destruct H as [v1' [v2' [same]]]. injection same. intros. subst. assumption.
+Qed.
+
+Fixpoint shape_sum_full Γ v A B ty (orig : has_vtype Γ v ty) {struct orig} :
+  ty = TyΣ A B ->
+  (exists name num, v = Var (name, num)) \/
+  (exists v1, v = Inl v1 /\ has_vtype Γ v1 A) \/
+  (exists v2, v = Inr v2 /\ has_vtype Γ v2 B).
+Proof.
+intros same.
+destruct orig. destruct H1; try discriminate.
++ clear shape_sum_full. left. exists name. exists num. reflexivity.
++ clear shape_sum_full. right. left. exists v. constructor. reflexivity.
+  inv same. assumption.
++ clear shape_sum_full. right. right. exists v. constructor. reflexivity.
+  inv same. assumption.
++ rewrite same in H2. apply subty_shape_sum in H2. 
+  destruct H2 as [A'' [B'' [pity]]]. subst. 
+  apply (shape_sum_full _ _ A'' B'') in H1. clear shape_sum_full. 
+  2: reflexivity. destruct H1.
+  - left. assumption.
+  - right. destruct H1.
+    * left. destruct H1. exists x. destruct H1. constructor. assumption.
+      apply TypeV. assumption. inv H0. assumption. eapply TypeVSubtype.
+      exact H3. destruct H2. assumption.
+    * right. destruct H1. exists x. destruct H1. constructor. assumption.
+      apply TypeV. assumption. inv H0. assumption. eapply TypeVSubtype.
+      exact H3. destruct H2. assumption.
+Qed.
+
+Lemma shape_sum_inl Γ v A B :
+  has_vtype Γ (Inl v) (TyΣ A B) -> has_vtype Γ v A.
+Proof.
+intro orig.
+apply (shape_sum_full _ _ A B) in orig as shape. 2: reflexivity.
+destruct shape.
++ destruct H as [name [num]]. discriminate.
++ destruct H.
+  - destruct H. destruct H. inv H. assumption.
+  - destruct H. destruct H. discriminate.
+Qed.
+
+Lemma shape_sum_inr Γ v A B :
+  has_vtype Γ (Inr v) (TyΣ A B) -> has_vtype Γ v B.
+Proof.
+intro orig.
+apply (shape_sum_full _ _ A B) in orig as shape. 2: reflexivity.
+destruct shape.
++ destruct H as [name [num]]. discriminate.
++ destruct H.
+  - destruct H. destruct H. discriminate.
+  - destruct H. destruct H. inv H. assumption.
+Qed.
+
+Fixpoint shape_prodmatch_full Γ c v x y c' C
+  (orig : has_ctype Γ c C) {struct orig} :
+  c = (ΠMatch v (x, y) c') ->
+  (exists A B, has_vtype Γ v (TyΠ A B) /\
+    has_ctype (CtxU (CtxU Γ A) B) c' C).
+Proof.  
+intros same. destruct orig. destruct H1; try discriminate.
++ clear shape_prodmatch_full. 
+  inv same. exists A. exists B. constructor; assumption.
++ apply (shape_prodmatch_full _ _ v x y c') in H1; clear shape_prodmatch_full. 
+  2: assumption. destruct H1 as [A' [B' [vty]]].
+  exists A'. exists B'. constructor. assumption.
+  apply TypeC.
+  - inv H1. assumption.
+  - assumption.
+  - eapply TypeCSubtype. exact H1. assumption.
+Qed.
+
+Fixpoint shape_prodmatch Γ v x y c C :
+  has_ctype Γ (ΠMatch v (x, y) c) C ->
+  (exists A B, has_vtype Γ v (TyΠ A B) /\  has_ctype (CtxU (CtxU Γ A) B) c C).
+Proof.
+intro orig. apply (shape_prodmatch_full _ _ v x y c) in orig.
+2: reflexivity. assumption.
+Qed.
+
+Fixpoint shape_summatch_full Γ c v xl cl xr cr C
+  (orig : has_ctype Γ c C) {struct orig} :
+  c = (ΣMatch v xl cl xr cr) ->
+  (exists A B, has_vtype Γ v (TyΣ A B) /\
+    has_ctype (CtxU Γ A) cl C /\ has_ctype (CtxU Γ B) cr C).
+Proof.  
+intros same. destruct orig. destruct H1; try discriminate.
++ clear shape_summatch_full. 
+  inv same. exists A. exists B. constructor. assumption.
+  constructor ; assumption.
++ apply (shape_summatch_full _ _ v xl cl xr cr) in H1;
+  clear shape_summatch_full. 2: assumption.
+  destruct H1 as [A' [B' [vty]]].
+  exists A'. exists B'. constructor. assumption.
+  inv H1. constructor; apply TypeC; auto.
+  - inv H3. assumption.
+  - eapply TypeCSubtype. exact H3. assumption.
+  - inv H4. assumption.
+  - eapply TypeCSubtype. exact H4. assumption.
+Qed.
+
+Fixpoint shape_summatch Γ v xl cl xr cr C :
+  has_ctype Γ (ΣMatch v xl cl xr cr) C ->
+  (exists A B, has_vtype Γ v (TyΣ A B) /\
+    has_ctype (CtxU Γ A) cl C /\ has_ctype (CtxU Γ B) cr C).
+Proof.
+intro orig. apply (shape_summatch_full _ _ v xl cl xr cr) in orig.
+2: reflexivity. assumption.
 Qed.
